gates/lean-axiom-probe.sh
@@ -83,6 +83,7 @@ THEOREMS=(
   "Thermite.EffectRows.outside_write_equal"
   "Thermite.LanguageCompleteness.expands_refl"
   "Thermite.LanguageCompleteness.expands_trans"
+  "Thermite.LanguageCompleteness.composeGuaranteeComplete"
   "Thermite.LanguageCompleteness.coreV1_expands_to_coreV2"
   "Thermite.LanguageCompleteness.narrowing_is_not_expansion"
   "Thermite.LanguageCompleteness.mutant_silent_narrowing_rejected"
